Handle non-expression rhs type

Optimizations/DSL/Canonicalization.thy
@@ -140,21 +140,21 @@ ML_file "rewrites.ML"
              
 subsubsection \<open>Semantic Preservation Obligation\<close>
 
-fun rewrite_preservation :: "IRExpr Rewrite \<Rightarrow> bool" where
-  "rewrite_preservation (Transform x y) = (y \<le> x)" |
-  "rewrite_preservation (Conditional x y conds) = (eval_condition conds \<longrightarrow> (y \<le> x))" |
+fun rewrite_preservation :: "(IRExpr, Result) Rewrite \<Rightarrow> bool" where
+  "rewrite_preservation (Transform x y) = (result_of y \<le> x)" |
+  "rewrite_preservation (Conditional x y conds) = (eval_condition conds \<longrightarrow> (result_of y \<le> x))" |
   "rewrite_preservation (Sequential x y) = (rewrite_preservation x \<and> rewrite_preservation y)" |
   "rewrite_preservation (Transitive x) = rewrite_preservation x"
 
 subsubsection \<open>Termination Obligation\<close>
 
-fun rewrite_termination :: "IRExpr Rewrite \<Rightarrow> (IRExpr \<Rightarrow> nat) \<Rightarrow> bool" where
-  "rewrite_termination (Transform x y) trm = (trm x > trm y)" |
-  "rewrite_termination (Conditional x y conds) trm = (eval_condition conds \<longrightarrow> (trm x > trm y))" |
+fun rewrite_termination :: "(IRExpr, Result) Rewrite \<Rightarrow> (IRExpr \<Rightarrow> nat) \<Rightarrow> bool" where
+  "rewrite_termination (Transform x y) trm = (trm x > trm (result_of y))" |
+  "rewrite_termination (Conditional x y conds) trm = (eval_condition conds \<longrightarrow> (trm x > trm (result_of y)))" |
   "rewrite_termination (Sequential x y) trm = (rewrite_termination x trm \<and> rewrite_termination y trm)" |
   "rewrite_termination (Transitive x) trm = rewrite_termination x trm"
 
-fun intval :: "Value Rewrite \<Rightarrow> bool" where
+fun intval :: "(Value, Value) Rewrite \<Rightarrow> bool" where
   "intval (Transform x y) = (x \<noteq> UndefVal \<and> y \<noteq> UndefVal \<longrightarrow> x = y)" |
   "intval (Conditional x y conds) = (eval_condition conds \<longrightarrow> (x = y))" |
   "intval (Sequential x y) = (intval x \<and> intval y)" |
